doot

_drafts/metatheory.lean
@@ -1,8 +1,91 @@
+-- import Init.Data.Nat
+/-
+A key piece of describing mathematical logic is the distinction between the object logic and the metalogic. This distinction is hard to keep clear in english sentences.
+I don't know the good way to make the leap of understanding. I think I have the spark of it, but not a full grokking.
 
-
-
+How does baby come to some understanding of words?
+How does a gradeschooler come to understand a "variable" or "polynomial". It's a gradual soak
+-/
+-- #print Nat
 example (x y : Nat) : x + y = y + x := by
-  rw [Nat.add_comm]
+  --omega
+  -- apply?
+  --exact?
+  exact Nat.add_comm x y
+  -- rw [Nat.add_comm]
+
+example (x y : Nat) : x + y = y + x + 0 := by
+  exact Nat.add_comm x y
+
+
+inductive Term where
+  | app : String -> Array Term -> Term
+
+inductive PeanoTerm where
+  | zero : PeanoTerm
+  | succ : PeanoTerm -> PeanoTerm
+  | plus : PeanoTerm -> PeanoTerm -> PeanoTerm
+
+-- numeral (sometimes an underbard, sometimes a little circle)
+def numeral ℕ -> PeanoTerm
+ | 0 => PeanoTerm.zero
+ | n + 1 => PeanoTerm.succ (numeral n)
+
+
+-- permute can freshen variables.
+def permute (x : String) (y : String) : Term -> Term
+  | Term.var z -> if z == x then Term.var y else if z == y then Term.var x else Term.var z
+  | Term.app f args => Term.app f (args.map (permute x y))
+
+-- chained permutations are a
+-- agda one that kmett referenced.
+
+
+/-
+It seems doofy, some forgettable shuffling. But it _is_ unavoidable (?)
+-/
+
+def interp : PeanoTerm -> Nat
+  | PeanoTerm.zero => 0
+  | PeanoTerm.succ n => 1 + interp n
+  | PeanoTerm.plus n m => interp n + interp m
+
+/-
+We can convert meta nat to object nat, but meta plus can't really be "seen" in the same way. And how much of this is special to how lean works.
+-/
+
+
+-- This is a set of terms.
+def is_zero (t : PeanoTerm) : Prop := interp t = 0
+
+
+
+
+
+partial def nat_interp : Term ->  Nat
+  | Term.app "+" args => args.foldl (init := 0) (fun acc arg => acc + nat_interp arg)
+  | Term.app "*" args => args.foldl (init := 1) (fun acc arg => acc * nat_interp arg)
+  | Term.app n _ => n.toNat!
+
+inductive Pf where
+  | ax : Term -> Pf
+  | mp : Pf -> Pf -> Pf
+
+/-
+"Truth" is a metalogical notion
+
+
+Carnap diagonalization
+Lob
+
+-/
+
+def true (p : Term) : Prop := true
+
+-- quoting
+
+-- trut predicate.
+
 
 
 def main : IO Unit := return ()
@@ -69,12 +152,6 @@ And they can be compared via the lean intermediary if you've given them semantic
 
 If you bottow your host powers, you kind of don't know what you're borrowing
 That's the beauty and danger of it
-
-
-
-
-
-
 
 
 -/
