_drafts/nand2lean.lean
@@ -1,0 +1,26 @@
+
+
+inductive Bnand : Bool -> Bool -> Bool -> Prop where
+  | nand_true_true : Bnand true true false
+  | nand_true_false : Bnand true false true
+  | nand_false_true : Bnand false true true
+  | nand_false_false : Bnand false false true
+--deriving instance Decidable for Bnand
+
+
+def Bnot (a b : Bool) : Prop := Bnand a a b
+
+-- This kind of let's me observe the not abstraction.
+--structure Bnot' (a b : Bool) : Prop where
+--  intro :: (h : Bnand a a b)
+
+example : Bnot true false := Bnand.nand_true_true
+example : Bnot false true := Bnand.nand_true_true
+
+
+/-
+This is all doofy.
+
+The exercise is kind of to just write an acceptor function or
+
+-/
