_drafts/boltmann_avo.md
@@ -1,0 +1,26 @@
+---
+
+title: The Boltzmann Constant kb is the inverse of Avogadro's number Na
+---
+
+No, I'm not insane.
+
+kb ~ 1/N
+
+On the face of this it is nonsense. The units don't work. Boltzmann's constant is unitful. Its value depends on your system of measure. Avogadro's constant converts between moles and a count. A mole is kind of like a dozen. It's almost more like changing the base of your number system than it is like changing units.
+
+But the point stands. The remarkable exponent of kb is -23 and the exponent of N is 23.
+Why?
+
+This is not exactly a coincidence. It is because we are human beings and defined our units of measure in terms of human quantities.
+
+The kg is approximately the units sausage are sold in. Meters are about how big horses are. We can feel fluctuations of temperature in the ballpark of 1 degree.
+
+Long before we were sure about atoms and exactly how big they might be, we were measuring temperatures and volumes and such.
+An inarguable fact is that kN = R, where R is the gas constant. R is 8.314. At the level of coarseness we are talking R is effectively 1 in human scale units. N is approximately the number of atoms in human scale stuff. Kb is
+
+So this fact that these constants are inverse is really a relative of the anthropic principle.
+
+pV = nRT
+
+Maybe another way of putting it is there is 1humanlength = 1meter  like how 1 lightmeter = c  
