_drafts/complexity.md
@@ -1,0 +1,49 @@
+---
+layout: post
+title: Complexity
+---
+
+[descriptive complexity](https://en.wikipedia.org/wiki/Descriptive_complexity_theory) queries in these logics when restricted to finite structures have this computational complexity
+
+Lower bounds
+Master theorem
+
+NP
+PSPACE
+
+Reductions
+
+<https://en.wikipedia.org/wiki/P_versus_NP_problem>
+
+Language
+
+<https://en.wikipedia.org/wiki/Blum_axioms>
+
+cook-levin is basically symbolically executing a turing machine using SAT.
+
+```python
+import turing
+
+```
+
+# Proof complexity
+<https://www.cs.cornell.edu/~sabhar/publications/iaspcmi-proofcomplexity00.pdf>
+Proofs are objects/
+co-NP = NP if proofs are small
+ASP might be nice for this.
+"transcript"
+
+<https://homes.cs.washington.edu/~beame/projects/proofcomplexity.html>
+ Size of resolu8tuion proofs?
+A strategy is to encode proofs as objects and sat search for them. Presumably proofs are too big for this to work well.
+
+Weak pigeonhole
+<https://people.cs.uchicago.edu/~razborov/files/php_survey.pdf>
+Pigeonhole =
+<https://x.com/codydroux/status/1712501511270420508> completeness is infinirary pigeonhole "Though in reverse mathematics, PH is much weaker than BW, mostly owing to the complexity of talking about reals. B-W is on par with some of the Ramsey theorems, apparently." Bolzano Weierstrauss
+
+<https://terrytao.wordpress.com/2007/05/23/soft-analysis-hard-analysis-and-the-finite-convergence-principle/>
+
+So there is sort of Soft / Analytic hiearchy
+Hard / Finitary / arithmetic hierarchy
+Complexity / polynomial hierachy
